Better `chan.select` model; regoose

new/golang/defn/chan.v
@@ -13,5 +13,18 @@ Axiom len : val.
 Axiom cap : val.
 Axiom for_range : val.
 
+(* FIXME: seal these functions *)
+Definition select_no_default : val :=
+  InjLV #().
+
+Definition select_default : val :=
+  λ: "f", InjR "f".
+
+Definition select_send : val :=
+  λ: "v" "ch" "f", InjL ("v", "ch", "f").
+
+Definition select_receive : val :=
+  λ: "ch" "f", InjR ("ch", "f").
+
 End defns.
 End chan.
